was geht das muss

HelloWorld_Proof.thy
@@ -4,77 +4,80 @@ begin
 
 text\<open>
   Apply some function \<^term>\<open>iofun\<close> to a specific world and return the new world
-  (discarding the result of \<^term>\<open>iofun\<close>).\<close>
-definition get_new_world :: "'\<alpha> io \<Rightarrow> \<^url> \<Rightarrow> \<^url>" where
-  "get_new_world iofun world = snd (Rep_io iofun world)"
+  (discarding the result of \<^term>\<open>iofun\<close>).
+\<close>
+definition exec :: "'\<alpha> io \<Rightarrow> \<^url> \<Rightarrow> \<^url>" where
+  "exec iofun world = snd (Rep_io iofun world)"
 
 text\<open>Similar, but only get the result.\<close>
-definition get_new_result :: "'\<alpha> io \<Rightarrow> \<^url> \<Rightarrow> '\<alpha>" where
-  "get_new_result iofun world = fst (Rep_io iofun world)"
+definition eval :: "'\<alpha> io \<Rightarrow> \<^url> \<Rightarrow> '\<alpha>" where
+  "eval iofun world = fst (Rep_io iofun world)"
 
-lemma get_new_world_Abs_io: "get_new_world (Abs_io f) world = snd (f world)"
-  by(simp add: get_new_world_def Abs_io_inverse)
+lemma exec_Abs_io: "exec (Abs_io f) world = snd (f world)"
+  by(simp add: exec_def Abs_io_inverse)
 
-lemma get_new_world_then:
-    "get_new_world (io\<^sub>1 \<then> io\<^sub>2) world = get_new_world io\<^sub>2 (get_new_world io\<^sub>1 world)"
-  and get_new_result_then:
-    "get_new_result (io\<^sub>1 \<then> io\<^sub>2) world = get_new_result io\<^sub>2 (get_new_world io\<^sub>1 world)"
-  by (simp_all add: get_new_world_def get_new_result_def bind_def Abs_io_inverse split_beta)
+lemma exec_then:
+    "exec (io\<^sub>1 \<then> io\<^sub>2) world = exec io\<^sub>2 (exec io\<^sub>1 world)"
+  and eval_then:
+    "eval (io\<^sub>1 \<then> io\<^sub>2) world = eval io\<^sub>2 (exec io\<^sub>1 world)"
+  by (simp_all add: exec_def eval_def bind_def Abs_io_inverse split_beta)
 
-lemma get_new_world_bind:
-    "get_new_world (io\<^sub>1 \<bind> io\<^sub>2) world = get_new_world (io\<^sub>2 (get_new_result io\<^sub>1 world)) (get_new_world io\<^sub>1 world)"
-  and get_new_result_bind:
-    "get_new_result (io\<^sub>1 \<bind> io\<^sub>2) world = get_new_result (io\<^sub>2 (get_new_result io\<^sub>1 world)) (get_new_world io\<^sub>1 world)"
-  by(simp_all add: get_new_world_def get_new_result_def bind_def Abs_io_inverse split_beta)
+lemma exec_bind:
+    "exec (io\<^sub>1 \<bind> io\<^sub>2) world = exec (io\<^sub>2 (eval io\<^sub>1 world)) (exec io\<^sub>1 world)"
+  and eval_bind:
+    "eval (io\<^sub>1 \<bind> io\<^sub>2) world = eval (io\<^sub>2 (eval io\<^sub>1 world)) (exec io\<^sub>1 world)"
+  by(simp_all add: exec_def eval_def bind_def Abs_io_inverse split_beta)
 
 text\<open>
   With the appropriate assumptions about \<^const>\<open>println\<close> and \<^const>\<open>getLine\<close>,
   we can even prove something.
 \<close>
-locale io_stdinout =
-  \<comment> \<open>We model stdin and stdout as part of the \<^typ>\<open>\<^url>\<close>.
+locale io_stdio =
+  \<comment> \<open>We model \<^verbatim>\<open>STDIN\<close> and \<^verbatim>\<open>STDOUT\<close> as part of the \<^typ>\<open>\<^url>\<close>.
      Note that we know nothing about \<^typ>\<open>\<^url>\<close>,
-     we just model that we can find stdin and stdout somewhere in there.\<close>
-  fixes get_stdout::"\<^url> \<Rightarrow> string list"
-  and get_stdin::"\<^url> \<Rightarrow> string list"
+     we just model that we can find \<^verbatim>\<open>STDIN\<close> and \<^verbatim>\<open>STDOUT\<close> somewhere in there.\<close>
+  fixes stdout_of::"\<^url> \<Rightarrow> string list"
+  and stdin_of::"\<^url> \<Rightarrow> string list"
 
-  \<comment> \<open>Assumptions about stdin:
-      Calling \<^const>\<open>println\<close> appends to the end of stdout and \<^const>\<open>getLine\<close> does not change anything.\<close>
-assumes get_stdout_println[simp]:
-    "get_stdout (get_new_world (println str) world) = get_stdout world@[String.explode str]"
-  and get_stdout_getLine[simp]:
-    "get_stdout (get_new_world getLine world) = get_stdout world"
+  \<comment> \<open>Assumptions about \<^verbatim>\<open>STDIN\<close>:
+      Calling \<^const>\<open>println\<close> appends to the end of \<^verbatim>\<open>STDOUT\<close> and \<^const>\<open>getLine\<close> does not change anything.\<close>
+assumes stdout_of_println[simp]:
+    "stdout_of (exec (println str) world) = stdout_of world@[String.explode str]"
+  and stdout_of_getLine[simp]:
+    "stdout_of (exec getLine world) = stdout_of world"
 
-  \<comment> \<open>Assumptions about stdin:
+  \<comment> \<open>Assumptions about \<^verbatim>\<open>STDIN\<close>:
       Calling \<^const>\<open>println\<close> does not change anything and \<^const>\<open>getLine\<close> removes the first element
-      from the stdin stream.\<close>
-  and get_stdin_println[simp]:
-    "get_stdin (get_new_world (println str) world) = get_stdin world"
-  and get_stdin_getLine:
-    "get_stdin world = inp#stdin \<Longrightarrow>
-     get_stdin (get_new_world getLine world) = stdin \<and> get_new_result getLine world = String.implode inp"
+      from the \<^verbatim>\<open>STDIN\<close> stream.\<close>
+  and stdin_of_println[simp]:
+    "stdin_of (exec (println str) world) = stdin_of world"
+  and stdin_of_getLine:
+    "stdin_of world = inp#stdin \<Longrightarrow>
+     stdin_of (exec getLine world) = stdin \<and> eval getLine world = String.implode inp"
 begin
 
   text\<open>Correctness of \<^const>\<open>main\<close>:
-    If stdout is initially empty and only \<^term>\<open>''corny''\<close> will be typed into stdin,
+    If \<^verbatim>\<open>STDOUT\<close> is initially empty and only \<^term>\<open>''corny''\<close> will be typed into \<^verbatim>\<open>STDIN\<close>,
     then the program will output: \<^term>\<open>[''Hello World! What is your name?'', ''Hello corny'']\<close>.
   \<close>
-  lemma assumes stdout: "get_stdout world = []" and stdin: "get_stdin world = [''corny'']"
-    shows "get_stdout (get_new_world main world) = [''Hello World! What is your name?'', ''Hello, corny!'']"
+  lemma
+    assumes stdout: "stdout_of world = []"
+         and stdin: "stdin_of world = [''corny'']"
+    shows "stdout_of (exec main world) = [''Hello World! What is your name?'', ''Hello, corny!'']"
   proof -
-    let ?world1="get_new_world (println (STR ''Hello World! What is your name?'')) world"
-    let ?world2="get_new_world getLine ?world1"
+    let ?world1="exec (println (STR ''Hello World! What is your name?'')) world"
+    let ?world2="exec getLine ?world1"
     from stdout have stdout_world2:
-      "get_stdout ?world2 = [''Hello World! What is your name?'']"
+      "stdout_of ?world2 = [''Hello World! What is your name?'']"
       apply simp
       apply code_simp
       done
-    from get_stdin_getLine[where stdin="[]", OF stdin] have stdin_world2:
-      "get_new_result getLine ?world1 = String.implode ''corny''"
-      by (simp add: get_stdin_getLine stdin)
+    from stdin_of_getLine[where stdin="[]", OF stdin] have stdin_world2:
+      "eval getLine ?world1 = String.implode ''corny''"
+      by (simp add: stdin_of_getLine stdin)
     show ?thesis
       unfolding main_def using stdout
-      apply(auto simp add: get_new_world_bind)
+      apply(auto simp add: exec_bind)
        apply code_simp
       apply (subst stdin_world2)
       apply (subst plus_literal.rep_eq)+
